\documentclass{article}
\usepackage[margin=1in]{geometry}
\usepackage{amsmath}
\usepackage{amssymb}
\usepackage{amsthm}
\usepackage{url}

% Environments

\newtheorem{theorem}{Theorem}
\newtheorem{proposition}[theorem]{Proposition}
\newtheorem{corollary}[theorem]{Corollary}
\newtheorem{lemma}[theorem]{Lemma}
\newtheorem{definition}[theorem]{Definition}
\newtheorem{conjecture}[theorem]{Conjecture}

\theoremstyle{definition}
\newtheorem{example}[theorem]{Example}

\numberwithin{theorem}{section}
\numberwithin{equation}{section}

\newcommand{\alg}{\mathcal{A}}
\newcommand{\sig}{\mathcal{S}}
\newcommand{\mono}{\mathcal{M}}
\newcommand{\sigmes}{\Lambda_{\mu^*}}
\newcommand{\salg}{$\sigma$-algebra}
\newcommand{\intd}{\, d}
%opening
\title{Assignment 1}
\author{Eric Luu}

\begin{document}

\maketitle
\section{Part 5}
\subsection{Question 1}


\begin{equation}
	g(x) := \tilde{g}(x) - \frac{1}{T} \int_{0}^{T} \tilde{g}(t) \, dt
\end{equation}

Then we have that for all $x$,
\begin{align*}
	\int_{x}^{x + T} g(t) \, dt &= \int_{x}^{x + T} \left(\tilde{g}(u) - \frac{1}{T} \int_{0}^{T} \tilde{g}(t) \, dt\right) \, du\\
	&= \int_{x}^{x + T} \tilde{g}(u)\, du - \int_{0}^{T} \tilde{g}(t) \, dt
\end{align*}
However, as $\tilde{g}(x)$ is $T$-periodic, it must hold that integration over any interval of length $T$ will yield the same result. Therefore, we have that
\begin{equation}
	\int_{x}^{x + T} \tilde{g}(u)\, du - \int_{0}^{T} \tilde{g}(t) \, dt = 0
\end{equation}

Now for any pair $p \leq q$ for any real number where $q > p + T$, we have that:
\begin{equation}
	\left| \int_{p}^{q} g(x) \, dx \right| = \left| \int_{p}^{q-T} g(x) \, dx +  \int_{q - T}^{q} g(x) \, dx\right| = \left| \int_{p}^{q-T} g(x) \, dx  \right|
\end{equation}
from above.

Therefore we can iterate this operation to find $q'$, where $\left| \int_{p}^{q} g(x) \, dx \right| = \left| \int_{p}^{q'} g(x) \, dx \right|$ and $p \leq q \leq p + T$. Then we have that from $T$-periodicity,
\begin{equation}
	\left| \int_{p}^{q'} g(x) \, dx \right| = \left| \int_{a}^{b} g(x) \, dx + \int_{c}^{d} g(x) \, dx \right|
\end{equation}
for some $ 0 \leq a \leq b \leq c \leq d \leq T$, by shuffling around the domains. We have that:
\begin{align*}
	\left| \int_{a}^{b} g(x) \, dx + \int_{c}^{d} g(x) \, dx \right| &\leq \left| \int_{a}^{b} g(x) \, dx \right| + \left| \int_{c}^{d} g(x) \, dx \right|\\
	&\leq  \int_{a}^{b} |g(x)| \, dx +\int_{c}^{d} |g(x)| \, dx\\
	&\leq \int_{0}^T |g(x)| \, dx
\end{align*}
But we have that $\int_{0}^T |g(x)| \, dx \leq T \max_{x \in [0, T]} |g(x)|$.

\subsubsection{Proving the integral}
Let $A$ be a measurable set where $\lambda(A) < \infty$ and $\chi_A$ be its associated characteristic function. Then we have that

\begin{equation}
	\int_{\mathbb{R}} \tilde{g}(nx) \chi_A \, dx = \int_{\mathbb{R}} \left(g(nx) + M\right) \chi_A \, dx
\end{equation}
We can split this integral into two sides. 

\begin{equation}
	\int_{\mathbb{R}} \left(g(nx) + M\right) \chi_A \, dx = \int_{\mathbb{R}}  g(nx) \chi_A \, dx + \int_{\mathbb{R}} M \chi_A \, dx = \int_{\mathbb{R}}  g(nx) \chi_A \, dx + M \lambda(A)
\end{equation}
What remains to show is that
\begin{equation}
	\lim_{n \rightarrow \infty} \int_{\mathbb{R}}  g(nx) \chi_A \, dx = 0. 
\end{equation}
PROVE HERE

\subsubsection{Extending to integrable functions}
As we have that $\int_{\mathbb{R}} \tilde{g}(nx) \chi_A \, dx = M \int_{\mathbb{R}} \chi(A) \, dx$, we have that for any $k \in \mathbb{R}$, $\int_{\mathbb{R}}\tilde{g}(nx) k \chi_A \, dx = k M \int_{\mathbb{R}} \chi_A  \, dx $ for any measurable $A$ by the linearity of the integral, and that for any measurable $A, B$, we have that
\begin{align*}
	\lim_{n \rightarrow \infty} \int_{\mathbb{R}} \tilde{g}(nx) (\chi_A + \chi_B) \, dx &= \lim_{n \rightarrow \infty} \int_{\mathbb{R}} \tilde{g}(nx) \chi_A \, dx + \lim_{n \rightarrow \infty} \int_{\mathbb{R}} \tilde{g}(nx) \chi_B \, dx\\
	&= M \int_{\mathbb{R}} \chi_A \, dx + M \int_{\mathbb{R}} \chi_B \, dx\\
	&= M \int_{\mathbb{R}} \chi_A + \chi_B \, dx 
\end{align*}
 by the linearity of the integral as well. So the property holds for any simple integrable function $f$.

Let $f$ be a integrable function and let $\left(  f_k \right)_k$ be a sequence of pointwise increasing simple functions converging to $f$. Then we have that
\begin{equation}
	h_k(x) := \lim_{n \rightarrow \infty} \tilde{g}(nx)f_k(x)
\end{equation}
is also a monotonically increasing function which converges to $h(x) := \lim_{n \rightarrow \infty} \tilde{g}(nx) f(x)$. Therefore by monotone convergence theorem, we have that:
\begin{align*}
	M \int_{\mathbb{R}} f(x) \, dx
	&= M \lim_{k \rightarrow \infty} \int_{\mathbb{R}} f_k(x) \, dx\\
	&= \lim_{k \rightarrow \infty} \lim_{n \rightarrow \infty} \int_{\mathbb{R}}  \tilde{g}(nx)f_k(x)\, dx\\
	&= \lim_{k \rightarrow \infty} \int_{\mathbb{R}}  h_k(x) \, dx\\
	&= \int_{\mathbb{R}} h(x) \, dx\\
	&= \int_{\mathbb{R}} \tilde{g}(nx)f_k(x) \, dx
\end{align*}
Thus shown.

\section{2}

\section{3}
Let $\omega = \mu + \nu$. We have that $\mu \leq \omega$ for all $\omega$. Then by Radon-Nicodym, there exists a $(\mu + \nu)$-measurable function $f$ with $0 \leq f \leq 1$ such that
\begin{equation}
	\mu(E) = \int_E f \, d\omega \qquad \forall E \in \mathcal{S}.
\end{equation} 
We will now use a fact from the proof of Radon-Nicodym that $\int_E f \, d\omega = \int_E f \, d\mu +  \int_E f \, d\nu$. Then we use the fact that $\mu(E) = \int_E 1 d\mu$ to get:
\begin{equation}
	\int_E 1 d\mu = \int_E f \, d\mu +  \int_E f \, d\nu \qquad \forall E \in \mathcal{S}.
\end{equation}
Then we move the $\int_E f \, d\mu$ term to the left hand side to have that:
\begin{equation}
	\int_E \left(1 - f\right) d\mu = \int_E f \, d\nu \qquad \forall E \in \mathcal{S}.
\end{equation}
where $f$ is $(\mu + \nu)$-measurable. 
\section{4}

\subsection{a}
We have that:
\begin{equation}
	\mu([0, \infty)) = \sum_{n = 1}^{\infty} \frac{1}{n^3} \int_{[n, n + 1)} x \, d\lambda \leq \sum_{n = 1}^{\infty} \frac{1}{n^3} (n + 1) = \sum_{n = 1}^{\infty} \frac{1}{n^2} + \sum_{n = 1}^{\infty} \frac{1}{n^3}
\end{equation}
However, we have that $\sum_{n = 1}^{\infty} \frac{1}{n^2}$ and $\sum_{n = 1}^{\infty} \frac{1}{n^3}$ are both finite, therefore $\mu([0, \infty)) < \infty$. 
We additionally have that
\begin{equation}
	\nu([1, \infty)) = \int_{[1, \infty)} x^{-2} \, d\lambda
\end{equation}
and using Riemannian integration and the fact that Riemannian and Lebesgue integration agree on continuous functions, we have that $\int_{[1, \infty)} x^{-2} \, d\lambda = \left[ -\frac{1}{x} \right]^\infty_{1} = 1$. Thus $\nu([1, \infty)) < \infty$ and $\mu$ and $\nu$ are finite measures. 
\subsection{b}
\paragraph{$\mu <<\lambda$}

We have that $\mu <<\lambda$. Let $A$ be a $\lambda$-null set. Then
\begin{equation}
	\mu(A) = \sum_{n = 1}^{\infty} \frac{1}{n^3} \int_{A\cap [n, n + 1)} x \, dx 
\end{equation}
but we have that for all $n$, $A\cap [n, n + 1)$ is also a null-set as it is a subset of $A$. Therefore, we can write
\begin{equation}
	\mu(A) = \sum_{n = 1}^{\infty} \frac{1}{n^3} \int_{\mathbb{R}} x \chi_{A\cap [n, n + 1)} \, dx 
\end{equation}
and we use the fact that $\int_{\mathbb{R}} x \chi_{A\cap [n, n + 1)} \, dx  = 0$ for all $n$ to yield $\mu(A) = 0$. Thus shown.

\paragraph{$\nu <<\lambda$}

Let $A$ be a $\lambda$-null set. Then:
\begin{equation}
	\nu(A) = \int_{A \cap [1, \infty)} x^{-2} \, dx
\end{equation}
but as $A \cap [1, \infty)$ is also a null-set as it is a subset of $A$, it holds that $\nu(A) = 0$ as well. 

\paragraph{$\lambda << \mu$}
It does not hold that $\lambda << \mu$. We have that:
\begin{equation}
	\mu([0, 1)) = 
	\sum_{n = 1}^{\infty} \frac{1}{n^3} \int_{[0, 1)\cap [n, n + 1)} x\, dx 
\end{equation}
but $[0, 1)\cap [n, n + 1) = \emptyset$ for all $n \geq 1$. Thus $\mu([0, 1)) = 0$, but $\lambda([0, 1)) = 1$. 

\paragraph{$\lambda << \nu$}
For a similar reason above, we have that

\begin{equation}
	\nu([0, 1)) = \int_{[0, 1) \cap [1 \infty)} x^{-2} \, dx\int_{\emptyset} x^{-2} \, dx = 0
\end{equation}
Thus shown.

\paragraph{$\mu << \nu$:}
Let $A$ be a null-set with respect to $\mu$. 

\paragraph{$\nu << \mu$:}
\end{document}