\documentclass[]{article}
\usepackage[margin=1in]{geometry}
\usepackage{amsmath}
\usepackage{amssymb}

\usepackage{hyperref}
\usepackage{cleveref}

\newcommand{\ops}{\overset{\text{ops}}{\leftrightarrow}}
\newcommand{\egf}{\overset{\text{egf}}{\leftrightarrow}}
%opening
\title{Assignment 3}
\author{Eric Luu}

\begin{document}

\maketitle
\section{Question 1}
\subsection{Part a}
We use the Taylor expansion of $\log(1 - x) = -x - \frac{x^2}{2} + O(x^3)$ with $\log(1 - n^{-1}) = -n^{-1} - \frac{n^{-2}}{2}+ O(n^{-3})$. We then have that:

\begin{align*}
	f(n) &= (n^2 + 7)\log(1 - n^{-1}) - n\\
	&= (n^2 + 7)\left(-n^{-1} - \frac{n^{-2}}{2} + O(n^{-3})\right) - n\\
	&= -n -\frac{1}{2} + O(n^{-1})- 7n^{-1} - \frac{7}{2}n^{-2} + O(n^{-3}) - n\\
	&= -2n -\frac{1}{2} + O(n^{-1})
\end{align*}
Therefore, we have that $f(n) = -2n -\frac{1}{2} + o(1)$, therefore $f(n) \sim -2n -\frac{1}{2}$. 
\subsection{Part b}
We use the same result above. We have that:

\begin{align*}
	f(n) &= (n^2 + 7)\log(1 - n^{-1}) + n - \frac{1}{2}\\
	&= (n^2 + 7)\left(-n^{-1} - \frac{n^{-2}}{2} + O(n^{-3})\right) + n - \frac{1}{2}\\
	&= -n -\frac{1}{2} + O(n^{-1})- 7n^{-1} - \frac{7}{2}n^{-2} + O(n^{-3}) + n - \frac{1}{2}\\
	&= -1 + O(n^{-1})
\end{align*}
Then we have that $f(n) \sim -1$. 

\section{Question 2}
\subsection{Part a}
We have that $f(n) = n^{n^2}(1 + \frac{1}{n})^{n^2}$. We have that $(1 + \frac{1}{n})^{n^2} = \exp\left(n^2 \log(1 + \frac{1}{n})\right)$ and we use the fact that $\log(1 + x) = x - \frac{1}{2}x^2 + O(x^3)$ when $x = o(1)$ to write $\log(1 + \frac{1}{n}) = \frac{1}{n} - \frac{1}{2}x^{-2} + O(n^{-3})$. Then we have that:
\begin{align*}
	\exp\left(n^2 \log(1 + \frac{1}{n})\right) &= \exp\left(n^2 \left(\frac{1}{n} - \frac{1}{2}x^{-2} + O(n^{-3}) \right)\right)\\
	&=  \exp\left( n  - \frac{1}{2}+ O(n^{-1})\right)\\
	&= \exp\left( n  - \frac{1}{2}+ o(1)\right)
\end{align*}
Therefore, we can write $f(n)$ as:
\begin{equation}
	f(n) = n^{n^2}e^{n - \frac{1}{2}}e^{o(1)}
\end{equation}
so $f(n) \sim n^{n^2}e^{n - \frac{1}{2}}$. 
Therefore, we have that $g(n) = n^{A(n)}e^{B(n)}$ where $A(n) = n^2$ and $B(n) = n - \frac{1}{2}$. 

\subsection{Part b}
We have that $f(n) - g(n) = (n + 1)^{n^2} - n^{n^2}e^{n - \frac{1}{2}} = n^{n^2}(1 + \frac{1}{n})^{n^2} - n^{n^2}e^{n - \frac{1}{2}}$. Factoring out the $n^{n^2}$ term, we have that $f(n) - g(n) = n^{n^2}\left((1 + \frac{1}{n})^{n^2} - e^{n - \frac{1}{2}} \right)$.

DO LATER, use more terms

\section{Question 3}
We can write the LHS as $\exp(f(n) \log(1 + o(1)))$. However, we have that $\log(1 + o(1)) = o(1)$, therefore we want that $\exp(f(n) o(1)) \sim 1$. Therefore, we want $f(n) o(1) = o(1)$, meaning that if we have $(1 + g(n))^{f(n)} \sim 1$, then $f(n)g(n) \sim 0$.  

\section{4}
\subsection{a}
We have that:
\begin{equation}
	\sum_{k = 0}^{J} \frac{n! n^k }{(n + k)! 2^k} = 
\end{equation}
\end{document}
